src/Constant.v
@@ -1,0 +1,160 @@
+Set Implicit Arguments.
+Require Import ZArith Psatz.
+Require Import Znumtheory.
+Require Import Classical.
+Require Import FunInd Recdef.
+Require Import List.
+Import ListNotations.
+Require Import MiniCooper.MyTactics.
+Require Import MiniCooper.LinSimpl.
+Open Scope list_scope.
+Open Scope Z_scope.
+
+(* ------------------------------------------------------------------------- *)
+(* Constants can be a combination of numeric literals and arbitrary expressions
+   (those are treated as abstract and kept in an environment). *)
+
+Notation var := nat.
+
+Notation environment := (var -> Z).
+
+Inductive constant :=
+| CAdd: constant -> constant -> constant
+| CMul: Z -> constant -> constant
+| CGround: Z -> constant
+| CAbstract: var -> constant.
+
+Fixpoint interpret_constant (cenv : environment) (c : constant) : Z :=
+  match c with
+  | CAdd c1 c2 =>
+    (interpret_constant cenv c1) + (interpret_constant cenv c2)
+  | CMul k c =>
+    k * (interpret_constant cenv c)
+  | CGround k =>
+    k
+  | CAbstract v =>
+    cenv v
+  end.
+
+(* Smart constructors for CAdd and CMul *)
+
+Function cadd (c1 c2 : constant) : constant :=
+  match (c1, c2) with
+  | (CGround k1, CGround k2) =>
+    CGround (k1 + k2)
+  | (CGround 0, _) =>
+    c2
+  | (_, CGround 0) =>
+    c1
+  | (_, _) =>
+    CAdd c1 c2
+  end.
+
+Lemma interpret_cadd:
+  forall cenv c1 c2,
+  interpret_constant cenv (cadd c1 c2) =
+  interpret_constant cenv c1 + interpret_constant cenv c2.
+Proof.
+  intros. functional induction (cadd c1 c2); simpl in *; eauto.
+Qed.
+
+Function cmul (k : Z) (c : constant) : constant :=
+  match c with
+  | CGround k' =>
+    CGround (k * k')
+  | _ =>
+    match k with
+    | 1 => c
+    | _ => CMul k c
+    end
+  end.
+
+Lemma interpret_cmul:
+  forall cenv k c,
+  interpret_constant cenv (cmul k c) =
+  k * interpret_constant cenv c.
+Proof.
+  intros. functional induction (cmul k c); cbn -[Z.mul] in *; eauto.
+Qed.
+
+(* ------------------------------------------------------------------------- *)
+(* Simplification procedure for constants. *)
+
+Module LinCst := LinSimpl (NatVar).
+
+Definition interp_var (cenv : environment) (v : var) :=
+  (* Use variable index [0] for the ground term *)
+  match v with
+  | O => 1
+  | S n => cenv n
+  end.
+
+(* Conversion from [constant] to [LinCst.t] *)
+
+Fixpoint linearize_constant (c : constant) : LinCst.lin :=
+  match c with
+  | CAdd c1 c2 =>
+    LinCst.add (linearize_constant c1) (linearize_constant c2)
+  | CMul k c =>
+    LinCst.mul k (linearize_constant c)
+  | CGround k =>
+    [(O, k)]
+  | CAbstract n =>
+    [(S n, 1)]
+  end.
+
+(* Conversion from [LinCst.t] to [constant] *)
+
+Definition linearized_to_constant (l : LinCst.lin) : constant :=
+  fold_right (fun '(v, k) acc =>
+    cadd acc
+      match v with
+      | O => CGround k
+      | S n => cmul k (CAbstract n)
+      end
+  ) (CGround 0) l.
+
+(* The simplification procedure *)
+
+Definition simpl_constant (c : constant) : constant :=
+  let l := linearize_constant c in
+  let l := LinCst.simpl l in
+  linearized_to_constant l.
+
+(* ------------------------------------------------------------------------- *)
+
+Lemma interpret_linearize_constant:
+  forall cenv c,
+  LinCst.interpret_lin (interp_var cenv) (linearize_constant c) =
+  interpret_constant cenv c.
+Proof.
+  induction c; simpl in *; eauto.
+  - rewrite LinCst.interpret_add. eauto.
+  - rewrite LinCst.interpret_mul, IHc. eauto.
+  - now destruct (cenv n).
+Qed.
+
+Local Arguments cmul : simpl never.
+
+Lemma interpret_linearized_to_constant:
+  forall cenv l,
+  interpret_constant cenv (linearized_to_constant l) =
+  LinCst.interpret_lin (interp_var cenv) l.
+Proof.
+  induction l as [|[? ?]]; eauto.
+  simpl. rewrite interpret_cadd, IHl.
+  destruct t; simpl.
+  - eauto with zarith.
+  - rewrite interpret_cmul. eauto with zarith.
+Qed.
+
+Lemma interpret_simpl_constant:
+  forall cenv c,
+  interpret_constant cenv (simpl_constant c) =
+  interpret_constant cenv c.
+Proof.
+  intros; unfold simpl_constant.
+  now rewrite interpret_linearized_to_constant,
+              LinCst.interpret_simpl,
+              interpret_linearize_constant.
+Qed.
